1.要证 $\bigcap_{i=1}^{+\infty}A_i\in\mathscr{F}_1$.

$\because A_i\in\mathscr{F}_1$, $i=1,2,....$

$\therefore A_i^c\in\mathscr{F}_1$, $i=1,2,....$

$\therefore \bigcup_{i=1}^{+\infty}A_i^c\in\mathscr{F}_1$

$\therefore (\bigcup_{i=1}^{+\infty}A_i)^c= \bigcap_{i=1}^{+\infty} A_i\in\mathscr{F}_1.$



2.

${\mathcal{F}}_{1}=\{(2,3-{\frac{1}{n}})\mid n=1,2,\cdots\}事件域$

$
A_{n}\in{\mathcal{F}}_{1},\;n=1,2,\cdots， A_{1}\subset A_{2}\subset\cdots\subset A_{n}$

$\bigcup_{i=1}^{+\infty}A_{i}=A_{n}\in{\mathcal{F}}_{1}$

$
\bigcup_{i=1}^{+\infty}A_{i}=(2,3)\notin{\mathcal{F}}_{1}$



3.

$\varphi(t) \stackrel{\Delta}{=} E e^{i t X} = \int_{-\infty}^{+\infty} e^{i t x} dF(x)$

$
\varphi(0) = E e^{i 0 X} = \int_{-\infty}^{+\infty} e^{i 0 x}  f(x) dx = \int_{-\infty}^{\infty} 1 \cdot  f(x) dx = 1$

$$|\varphi(t)|\stackrel{\Delta}{=}|E e^{i t X}|=\left|\int_{-\infty}^{+\infty}e^{itx}f(x)dx\right|\leq\int_{-\infty}^{+\infty}|e^{itx}|f(x)dx\leq \int _ { - \infty } ^ { + \infty } 1 \cdot f ( x ) d x = 1 .$$



4.

$\sum_{l=1}^{n}\sum_{k=1}^{n}\varphi(t_{k}-t_{l})z_{k}\overline{z_{l}}$

$
=\sum_{l=1}^{n}\sum_{k=1}^{n}\mathrm{E}e^{i(t_{k}-t_{l})X}z_{k}\overline{z_{l}}$

$=\sum_{l=1}^{n}\sum_{k=1}^{n}\mathrm{E}e^{-it_{k}X}e^{-it_{l}X}z_{k}\overline{z_{l}}$

$=\mathrm{E}(\sum_{l=1}^{n}e^{-it_{l}X}\overline{z_{l}})(\sum_{k=1}^{n}e^{-it_{k}X}z_{k})$

$=E\left|\sum_{k=1}^{n}e^{it_kX}\cdot z_k\right|^2\geq0.$



5.

$\varphi(t)=E e^{itX}=Ee^{it(X_{1}+\ldots+X_{n})}$
$
=E(e^{itX_{1}}\ldots e^{itX_{n}})$
$=Ee^{itX_{1}}\cdot Ee^{itX_{2}}\ldots Ee^{itX_{n}}$
$
=\varphi_{1}(t)\cdot\varphi_{2}(t)\ldots\varphi_{n}(t)$



6.

$X \sim N(a,\sigma^2).$ 求 $X$ 的特征函数

$$\int_{-\infty}^{+\infty}\frac{1}{\sqrt{2\pi}}e^{-\frac{u^2}{2}}du=1$$

$\int_{-\infty}^{+\infty}e^{-\frac{u^2}{2}}du=\sqrt{2\pi}$

$\phi(t)=E e^{itX}=\int_{-\infty}^{+\infty} e^{itx} \frac{1}{\sqrt{2\pi} \sigma} e^{-\frac{(x-a)^2}{2\sigma^2}} dx$
$令 u=\frac{x-a}{\sigma}$
$=\int_{-\infty}^{+\infty} e^{it(a+\sigma u)} \frac{1}{\sqrt{2\pi }\sigma} e^{-\frac{u^2}{2}} \sigma du$
$=\frac{1}{\sqrt{2\pi}} e^{iat} \int_{-\infty}^{+\infty} e^{-\frac{u^2}{2}+it\sigma u} du$

$$=\frac{1}{\sqrt{2\pi}}e^{iat}\int_{-\infty}^{+\infty}e^{-\frac{(u-it\delta)^2}{2}}e^{-\frac{\sigma^2t^2}{2}}du$$

$$= \frac{1}{\sqrt{2\pi}}e^{ia t-\frac{\sigma^2t^2}{2}}\int_{-\infty}^{+\infty}e^{-\frac{(u-it\sigma)^2}{2}}d(u-it\sigma)$$

$=e^{ia t-\frac{\sigma^2t^2}{2}}$

$\phi'(t)=e^{iat-\frac{\sigma^2t^2}{2}}\cdot (ia-\sigma^2t)$
$\phi'(0)=ia=iEX$



7.

$X \sim N(a,\sigma^2), \quad \varphi(t) = e^{i\alpha t - \frac{\sigma^2 t^2}{2}}$

$$X \sim N(a,B), \quad \varphi(t) = e^{ia t' + \frac{tBt'}{2}}$$



8.

$P(Y=y_j|X=x_i)=\frac{P(X=x_i,Y=y_j)}{P(X=x_i)},\quad j=1,2,\cdots$

$
E(Y|X=x_i)=\sum_j y_jP(Y=y_j|X=x_i)$



9.

​     $\mathrm{D}_{X}(t)=\mathrm{E} X_{(t)}^{2}-\left(\mathrm{E} X_{(t)}\right)^{2}$

$
=\psi_{X}(t)-m_{X(t)}^{2}$

​      $\mathrm{C}_{X}\left(t_{1}, t_{2}\right)=\mathrm{Cov}\left(X\left(t_{1}\right), X\left(t_{2}\right)\right)$

$
=\mathrm{E}\left(X\left(t_{1}\right)-m_{X\left(t_{1}\right)}\right)\left(X\left(t_{2}\right)-m_{X\left(t_{2}\right)}\right)$

$=\mathrm{E} X\left(t_{1}\right) X\left(t_{2}\right)-\mathrm{E} X\left(t_{1}\right) \mathrm{E} X\left(t_{2}\right)$

​      $
\mathrm{R}_{X}\left(t_{1}, t_{2}\right)(自相关函数)=\mathrm{E} X\left(t_{1}\right) X\left(t_{2}\right)$



10.

​     $m_{X}(t)=E X(t)=E {a \cos \left(\omega_{0} t+\Phi\right)}{}$
$
=\int_{0}^{2 \pi} a \cos \left(\omega_{0} t+\varphi\right) \cdot \frac{1}{2 \pi} d \varphi .$
$=\left.\frac{d}{2 \pi} \sin \left(\omega_{0} t+\varphi\right)\right|_{0} ^{2 \pi}$
$
=0$

   $R_X(t_1,t_2)=EX(t_1)X(t_2)=E\left[{a^2}\cos(\omega_0t_1+\Phi)\cos(\omega_0t_2+\Phi)\right]$
$
={a}^2\int_0^{2\pi}\cos(\omega_0t_1+\phi)\cos(\omega_0t_2+\phi)\cdot\frac{1}{2\pi}d\phi$
$=\frac{{a}^2}{2\pi}\cdot\frac{1}{2}\int_0^{2\pi}\left[\cos(\omega_0(t_1+t_2)+2\phi)+\cos\omega_0(t_1-t_2)\right]d\phi$

$=\frac{a^2}{4\pi}\left[\frac{1}{2}\sin(\omega_0(t_1+t_2)+2\varphi)|_{0} ^{2 \pi}+2\pi\cos\omega_0(t_1-t_2)\right]$
$
=\frac{a^2}{2}\cos\omega_0(t_1-t_2)$

$$D_X(t)=\psi_{X}(t)-m_{X(t)}^{2}=R_X(t,t)-m_{X(t)}^{2}=\frac{a^2}{2}$$



11.

$任意t_1, \cdots t_n$ 求 $\zeta(t_1), \cdots \zeta(t_n)$ 的密度函数

均值向量 $M_\zeta=(M_\zeta(t_1), \cdots M_\zeta(t_n))=(0, \cdots 0)$

$(\zeta(t_1), \cdots \zeta(t_n))=(t_1\xi+\eta, t_2\xi+\eta, \cdots t_n\xi+\eta)$

$=(\xi, \eta)\begin{pmatrix} t_1 & t_2 & \cdots & t_n \\ 1 & 1 & \cdots & 1  \end{pmatrix}$ (是否正定?)

X～N($a$，$B$)
$Y=XA$，若$A^TBA$正定，则Y～N($aA$，$A^TBA$)

$A^T B A=\begin{pmatrix} t_1 & 1\\ t_2  & 1\\ \vdots &\vdots \\ t_n  & 1\end{pmatrix} \begin{pmatrix} 1 & 0 \\ 0 & 1 \end{pmatrix}\begin{pmatrix} t_1 & t_2 & \cdots & t_n \\ 1 & 1 & \cdots & 1  \end{pmatrix} $

 n>2， 乘积的秩小于等于分量的秩

$\varphi(t_1,\ldots t_n)=e^{i{m_\zeta}^T-\frac{1}{2}tCt^T}$



12.

$\Rightarrow C(s,t)=EX(s)X(t)-EX(s)EX(t)$
$
=EX(s)EX(t)-EX(s)EX(t)=0$

$\Leftarrow \forall t_1,\ldots t_n\in T,(X_{(t_1)},\ldots X_{(t_n)})的特征函数\varphi(u_1,\ldots u_n)$
$
为\varphi(u_1,\ldots u_n)=e^{im_Xu^T-\frac{1}{2}uCu^T}$

${m}_X=({m}_x(t_1),\ldots,{m}_x(t_n))$
$
{u}=(u_1,\ldots,u_n)$

$$C=\begin{pmatrix}C_X(t_1,t_1)&0&\cdots&0\\0&C_X(t_2,t_2)&\cdots&0\\\vdots&\vdots&\vdots&\vdots\\0&0&\cdots&C_X(t_n,t_n)\end{pmatrix},$$



$\varphi(u_1,\cdots u_n)=e^{i\sum_{j=1}^{n}m_{x}(t_j)u_{j}-\frac{1}{2}\sum_{j=1}^{n}C(t_{j},t_{j})u_{j}^{2}}$

$
=\Pi_{j=1}^ne^{im_{x}(t_j)u_{j}-\frac{1}{2}C(t_{j},t_{j})u_{j}^{2}}$
$=\varphi(t_1)\cdots\varphi(t_n)$



13.

$\left({E}XY\right)^2 \leq {E}X^2 \cdot {E}Y^2$

$
\left(\int f(x)g(x)dx\right)^2 \leq \left[\int f^2(x)dx\right]\left[\int g^2(x)dx\right]$

$R_X(t_1,t_2) ={E}X(t_1)X(t_2) \leq \left({E}X^2(t_1)\right)^{1/2}\left({E}X^2(t_2)\right)^{1/2} < +\infty$

$
C_X(t_1,t_2) = R_X(t_1,t_2) - m_X(t_1)m_X(t_2)$



14.

​	${{ \sum _ { k = 1 } ^ { n } \sum _ { j = 1 } ^ { n } R _ { X } ( \tau _ { k } , \tau _ { j } ) z _ { k } \overline { z _ { j } } }  }$
$
= { } \sum _ { k = 1 } ^ { n } \sum _ { j = 1 } ^ { n } E X ( \tau _ { k } ) X ( \tau _ { j } ) z _ { k } \overline { z _ { j } }$
$= E \sum _ { k = 1 } ^ { n } \sum _ { j = 1 } ^ { n } X ( \tau _ { k } ) X ( \tau _ { j } ) z _ { k } \overline { z _ { j } }$
$
= E \left( \sum _ { j = 1 } ^ { n }  X ( \tau _ { j } ) \overline { z _ { j } } \right) \left( \sum _ { k = 1 } ^ { n }  X ( \tau _ { k } ) z _ { k } \right)$

$≥ 0$



15.

$要证 P(|X-Y|=C)=1 \Longleftrightarrow D|X-Y|=0$
$\because D|X-Y| = E|X-Y|^2 - (E|X-Y|)^2$
$其中 E|X-Y|^2 = E|(X_n-X)-(X_n-Y)|^2$
$\leqslant E|X_n-X|^2 + E|X_n-Y|^2 + 2E|X_n-X||X_n-Y|$
$\leqslant E|X_n-X|^2 + E|X_n-Y|^2 + 2[E|X_n-X|^2]^{\frac{1}{2}}[E|X_n-Y|^2]^{\frac{1}{2}}$



16.

$\lim_{n \to +\infty}{E} |X_n - X|^2 = 0$
$
|{E} X_n - {E} X| = |{E} (X_n - X) \cdot 1| \leq ({E} |X_n - X|^2)^{\frac{1}{2}} ({E} 1^2)^{\frac{1}{2}}$
${E} XY \leq ({E} X^2)^{\frac{1}{2}} ({E} Y^2)^{\frac{1}{2}} \xrightarrow{n \to +\infty} 0$

$\lim\limits_{n\to\infty} EX_n = E \lim\limits_{n\to\infty} X_n.$



17.

$\lim\limits_{\begin{array}{c}m\to\infty\\n\to\infty\end{array}}E(X_mY_n)=E(XY)=E(\lim\limits_{\begin{array}{c}m\to\infty\\\end{array}}X_m\cdot\lim\limits_{\begin{array}{c}n\to\infty\end{array}}Y_n)$

$
|E(X_mY_n)-E(XY)|=|E(X_mY_n-XY)|$

$\leqslant E|(X_m-X)(Y_n-Y)|+E|(X_m-X)Y|+E|(Y_n-Y)X|$

$\leqslant\sqrt{E(X_m-X)^2}\sqrt{E(Y_n-Y)^2}
+\sqrt{E(X_m-X)^2}\sqrt{E(Y)^2}+\sqrt{E(Y_n-Y)^2}\sqrt{E(X)^2}\xrightarrow{n \to +\infty} 0$
$
\lim\limits_{m\to\infty}E(X_m-X)=0$
$\lim\limits_{n\to\infty}E(Y_n-Y)=0$



18.

$\lim _ { n \rightarrow \infty }  { E } \left| a _ { n } X - 0 \right| ^ { 2 } = \lim _ { n \rightarrow \infty }  { E } \left| a _ { n } X \right| ^ { 2 }$
$
= \lim _ { n \rightarrow \infty } a _ { n } ^ { 2 } \cdot  { E } X ^ { 2 }$
$\rightarrow 0$



19.

$\lim\limits_{\begin{array}{c}m\to\infty\\n\to\infty\end{array}}E|X_{m}-X_{n}|^{2}$

$=\lim\limits_{\begin{array}{c}m\to\infty\\n\to\infty\end{array}}E[(X_{m}-X)-(X_{n}-X)]^{2}$

$\leqslant\lim\limits_{\begin{array}{c}m\to\infty\\n\to\infty\end{array}}[E|X_{m}-X|^{2}+E|X_{n}-X|^{2}+2E|X_{m}-X||X_{n}-X|]=0$



20.

$\left|f(u)-f(v)\right|\leq M\left|u-v\right|$
$
f(X_n)\overset{L^2}{\to}f(X)\qquad n\to\infty$

$\left|f(X_n)-f(X)\right|^2\leq M^2\left|X_n-X\right|^2$

$\lim_{n\to\infty}{E}|f(X_n)-f(X)|^2$
$\leq\lim_{n\to\infty}{E}M^2|X_n-X|^2$
$=M^2\lim_{n\to\infty}{E}|X_n-X|^2$
$=0$

21.

$证明\lim_{n \to \infty} E|X_n - \mu|^2 = 0$
$E|X_n - \mu|^2$
$= E|\frac{1}{n} \sum_{i=1}^{n} Y_i - \mu|^2$
$= \frac{1}{n^2} E|\sum_{i=1}^{n} Y_i - n\mu|^2$
$
= \frac{1}{n^2} E|\sum_{i=1}^{n} (Y_i - \mu)|^2$

$
\sum_{i}\sum_{j}E(Y_{i}-\mu)(Y_{j}-\mu),i\neq j$
$=\sum_{i}\sum_{j}E(Y_{i}-\mu)E(Y_{j}-\mu)$
$
=0$

故上式$= \frac{1}{n^2} \sum_{i=1}^{n} E(Y_i - \mu)^2$

$E(Y_{i}-\mu)^{2}$
$
=D(Y_{i}-\mu)+[E(Y_{i}-\mu)]^{2}$
$=\sigma^{2}+0$

故上式$= \frac{\sigma^{2} }{n}\xrightarrow{n \to +\infty} 0$

 

22.

$\lim _ { \substack { t _ { 1 } \rightarrow t _ { 0 } \\ t _ { 2 } \rightarrow t _ { 0 } } } R _ { X } ( t _ { 1 } , t _ { 2 } ) = \lim _ { \substack { t _ { 1 } \rightarrow t _ { 0 } \\ t _ { 2 } \rightarrow t _ { 0 } } } E X ( t_1 ) X ( t_2 )$

$= \lim_{t_1 \to t_0} X (t_1) \cdot \lim_{t_2 \to t_0} X (t_2)$

$= E X (t_0) X (t_0) $ 

$= R_x (t_0, t_0) $

证 $E|X(t)-X(t_0)|^2$  
$=E X(t)^2+E X(t_0)^2-2E X(t) X(t_0)$  
$=R_X(t,t)+R_X(t_0,t_0)-2R_X(t,t_0)$  
$\xrightarrow{t \to t_0} R_X(t_0,t_0)+R_X(t_0,t_0)-2R_X(t,t_0)=0$



23.

已知 $\lim_{h \to 0} \frac{X(t+h) - X(t)}{h} = X'(t)$

证明 $\lim_{h \to 0} X(t+h) = X(t)$

$\lim_{h \to 0} E|X(t+h) - X(t)|^2 = \lim_{h \to 0} h^2 E\left|\left(\frac{X(t+h) - X(t)}{h} - X'(t)\right) + X'(t)\right|^2$

$= h^2 \lim_{h \to 0} E\left|\frac{X(t+h) - X(t)}{h} - X'(t) \right|^2 + E X'(t)^2 + 2 E \left(\frac{X(t+h) - X(t)}{h} - X'(t)\right) X'(t)$

柯西施瓦兹$\to 0$



24.

$\int_a^b\int_a^bR_X(s,t)dsdt\text{ 存在} \Rightarrow \int_a^bX(t)dt\text{ 存在}$
$
\because X(t) \text{ 在 } [a,b] \text{ 均方连续}$
$\therefore \lim\limits_{\begin{array}{c}s\to s_0\\t\to t_0\end{array}}R_X(s,t) =  \lim\limits_{\begin{array}{c}s\to s_0\\t\to t_0\end{array}}E[X(s)X(t)] = E[\lim_{s\to s_0}X(s)\lim_{t\to t_0}X(t)]$
$
= E[X(s_0)X(t_0)] = R_X(s_0,t_0)$
$\therefore \int_a^b\int_a^bR_X(s,t)dsdt\text{ 存在}$



25.

$E\int\limits_{a}^{b}f(t)X(t)\;dt$

$=E\left(\lim\limits_{\Delta\to 0}\sum\limits_{k=1}^{n}f(u_k)X(u_k)\;(t_k-t_{k-1})\right)$

$=\lim\limits_{\Delta\to 0}\sum\limits_{k=1}^{n}f(u_k)E(X(u_k))\;(t_k-t_{k-1})$

$=\lim\limits_{\Delta\to 0}\sum\limits_{k=1}^{n}f(u_k)\;m_X(u_k)\;(t_k-t_{k-1})$

$=\int\limits_{a}^{b}f(t)\;m_X(t)\;dt.$



26.

例：设 $X(t) = \sin At$，其中 $A$ 为 r.v.，$E A^4 < +\infty$，

证：$X'(t) = A \cos At$

$E |\frac{X(t+h)-X(t)}{h}-A \cos A t |^2$
$= E | \frac{\sin A (t+h)-\sin A t}{h}-A \cos A t |^2$
$= E| \frac{\sin A t \cos A h + \cos A t \sin A h-\sin A t-A h \cos A t}{h}|^2$

$= E| \frac{\sin A t(cos A h -1) +\cos A t (\sin A h-A h)}{h}|^2$

$\leq 2 E [\frac{(\sin A t)^2 (A h)^4 + (\cos A t)^2 (A h)^4}{h^2}]$

$= 2 h^2 \cdot E [(\sin A t)^2 A^4 + (\cos A t)^2 A^4]$

$= 2 h^2 \cdot E A^4 \xrightarrow{h \to 0} 0$



27.

$例:设X(t)=2A^2t, A为r.v., EA^4<+∞, 求∫^t_0X(s)ds.$
$解: R_X(s,t)=EX(s)X(t)=E(2A^2s·2A^2t)=E(4A^4st)
=4·EA^4·st$
$∫^b_a∫^b_aR_X(s,t)dsdt=∫^b_a∫^b_astdsdt存在$
$\therefore \int_{0}^{t} X(s) \mathrm{d}s 存在. 0=t_{0}< t_{1} \cdots t_{n}=t$
$
\int_{0}^{t} X(s) \mathrm{d}s $$= \lim_{\Delta \to 0} \sum_{k=1}^{n}  X(u_{k}) (t_{k} - t_{k-1})$

$ = \lim_{\Delta \to 0} \sum_{k=1}^{n}2 A^{2} u_{k} (t_{k} - t_{k-1})$
$= \lim_{\Delta \to 0}  2 A^{2} \sum_{k=1}^{n} \frac{1}{2} (t_{k} + t_{k-1}) (t_{k} - t_{k-1})$
$
= \lim_{\Delta \to 0}  2 A^{2} \frac{1}{2} (t^{2} - 0^{2})$
$= \lim_{\Delta \to 0} A^{2} t^{2}$
$
= A^{2} t^{2}$

$\int_{0}^{t}X(s)ds$
$
= \int_{0}^{t}2A^2sds$
$= A^2\int_{0}^{t}2sds$
$
= A^2t^2$



28.

设 $X_t = Ae^{-3t}\cos 2t$, 其中A为r.v., 且 $EA = 5$, $DA = 1$, 求 $Y(t) = \int_0^t X(\tau) d\tau$ 的均值函数

$$Y(t)=A\int_{0}^{t}e^{-3\tau}\cos(2\tau)d\tau$$

计算积分:
设$
I=\int_{0}^{t}e^{-3\tau}\cos(2\tau)d\tau$

- 第一次分部积分:
$u=\cos(2\tau), dv=e^{-3\tau}d\tau, du=-2\sin(2\tau)d\tau, v=-\frac{1}{3}e^{-3\tau}$
$
I=-\frac{1}{3}e^{-3\tau}\cos(2\tau)-\frac{2}{3}\int_{0}^{t}e^{-3\tau}\sin(2\tau)d\tau$
- 第二次分部积分:
对
$\int_{0}^{t}e^{-3\tau}\sin(2\tau)d\tau, u=\sin(2\tau), dv=e^{-3\tau}d\tau, du=2\cos(2\tau)d\tau, v=-\frac{1}{3}e^{-3\tau}$
$
\int_{0}^{t}e^{-3\tau}\sin(2\tau)d\tau=-\frac{1}{3}e^{-3\tau}\sin(2\tau)+\frac{2}{3}\int_{0}^{t}e^{-3\tau}\cos(2\tau)d\tau$

- 求解$I$:
$
I=-\frac{1}{3}e^{-3\tau}\cos(2\tau)-\frac{2}{3}\left(-\frac{1}{3}e^{-3\tau}\sin(2\tau)+\frac{2}{3}I\right)$
$\frac{13}{9}I=-\frac{1}{3}e^{-3\tau}\cos(2\tau)+\frac{2}{9}e^{-3\tau}\sin(2\tau)$
$
I=\frac{e^{-3\tau}}{13}(2\sin(2\tau)-3\cos(2\tau))|_{0}^{t}=\frac{e^{-3t}}{13}(2\sin(2t)-3\cos(2t))+\frac{3}{13}$

求均值函数:
$$E[Y(t)]=E[A]\int_{0}^{t}e^{-3\tau}\cos(2\tau)d\tau$$
已知$
E[A]=5$, 则
$$E[Y(t)]=5\times\left(\frac{e^{-3t}}{13}(2\sin(2t)-3\cos(2t))+\frac{3}{13}\right)=\frac{5}{13}\left(e^{-3t}(2\sin(2t)-3\cos(2t))+3\right)$$

29.

$m_{X}(t)=E X(t)=\int_{-\infty}^{+\infty} x d F(x, t)=\int_{-\infty}^{+\infty} x d F(x, t+\tau)=m_{X}(t+\tau)$

$m_{X}(t)=m_{X}$

$R_{X}(t, t+\tau)=E X(t) X(t+\tau)=\int_{-\infty}^{+\infty} \int_{-\infty}^{+\infty} x_{1} x_{2} d F\left(x_{1}, x_{2} ; t, t+\tau\right)$

$=\int_{-\infty}^{+\infty} \int_{-\infty}^{+\infty} x_{1} x_{2} d F\left(x_{1}, x_{2} ; 0, \tau\right)$

$=R_{X}(0, \tau)=R_{X}(\tau)$



30.

$
\begin{array}{r} {N(0,\sigma^{2}) \quad m_X(n)=EX(n)=0 \quad \text{常数}} \end{array}$
$\begin{array}{r} { \rho=0=\frac{\operatorname{Cov}(X(n),X(n+m))}{\sqrt{DX(n)} \cdot \sqrt{DX(n+m)}}.} \end{array}$
$EX(n)X(n+m)={\operatorname{Cov}(X(n),X(n+m))}=0$
$
\begin{array}{r} {EX(n)^{2}=DX(n)+(EX(n))^{2}=\sigma^{2}} \end{array}$
$\begin{array}{r} {R_{X}(n,n+m)=EX(n)X(n+m)=\left\{\begin{array}{ll} {0,} & {m\neq0} \\ {\sigma^{2},} & {m=0} \end{array}\right.} \end{array}$

31.

$Z(n) = \sum_{k=-\infty}^{+\infty} a_k X(n-k)$

$=\lim_{N\to+\infty} \sum_{k=-N}^{N} a_k X(n-k)$   
$\sum_{k=-N}^{N} a_k X(n-k) = Z^{(N)}$
$先说明\lim_{N\to\infty} Z_n ^{(N)}存在$
$
\lim_{n\to\infty} X_n 存在 \Leftrightarrow \lim\limits_{\begin{array}{c}m\to\infty\\n\to\infty\end{array}}(X_n-X_m)=0$
$
即说明\lim\limits_{\begin{array}{c}M\to\infty\\N\to\infty\end{array}}(Z_n^{(N)}-Z_n^{(M)})=0$

$
即证\lim\limits_{\begin{array}{c}M\to\infty\\N\to\infty\end{array}}E|Z_n^{(N)}-Z_n^{(M)}|^2=0$

$设N>M$
$E\left|Z_{(n)}^{(N)}-Z_{(n)}^{(M)}\right|^{2}$

$=E\left|\sum_{m<|k|\leq N}a_{k} X_{(n-k)}\right|^{2}$
$=E\left(\sum_{m<|k|\leq N}Z_{(n)}^{(k)}\right)\left(\sum_{m< |l|\leq N}Z_{(n)}^{(l)}\right)$

$=E\left(\sum_{M<|k|\leq N}a_{k}X(n-k)\right)\left(\sum_{M<l\leq N}a_{l}X(n-l)\right)$

$
=\sum_{M<|k|\leq N}a_{k}^{2}E\left(X(n-k)^{2}\right)=\sigma^{2}\sum_{M<|k|\leq N}a_{k}^{2}$

$\sum_{M<|k|\leq N}a_k^2 \xrightarrow{M \to \infty, N \to \infty}0$?

$
= \sum_{M<K\le N}a_k^2 + \sum_{-N\le K< -M}a_k^2$

$\le \sum_{K> M}a_k^2 + \sum_{K< M}a_k^2$

$
\xrightarrow{M \to \infty}0+0=0$

$EZ(n)=E\sum_{k=-\infty}^{+\infty}a_{k}X(n-k)=E\lim_{N\to\infty}\sum_{k=-N}^{N}a_{k}X(n-k)$
$
=0$
$R_{X}(n,n+j)=EZ(n)Z(n+j)$

$
=E\sum_{k=-\infty}^{+\infty}a_{k}X(n-k)\sum_{\ell=-\infty}^{+\infty}a_{\ell}X(n+j-\ell)$

$=\sum_{k=-\infty}^{+\infty}\sum_{\ell=-\infty}^{+\infty}a_{k}a_{\ell}E[X(n-k)X(n+j-\ell)]$

$$\begin{array}{r} \mathrm{E}\left[X(n-k)X(n+j-\ell)\right]= \begin{cases} 0,&\ell\neq j+k.\\ \sigma^2,&\ell=j+k. \end{cases} \end{array}$$

$$=\sum_{k=-\infty}^{+\infty}a_{k}a_{j+k}\sigma^{2}={R_X}(u)$$



32.

$E X(n)=E\xi \cos n w+E\eta \sin n w=0=m_X$
$
R_{X}(n, n+m)=E X_{(n)} X_{(n+m)}$
$=E\left(\xi \cos n w+\eta \sin n w\right)\left(\xi \cos (n+m) w+\eta \sin (n+m) w\right)$
$
=E\left[\xi^{2} \cos n w \cos (n+m) w+\eta^{2} \sin n w \cdot \sin (n+m) w\right]$
$=\sigma^{2} \cos m w=R_{X}(m)$

33.

34.

$$E\xi_k^2=\sigma_k^2$$
$$
\xi_k e^{in\omega_k}=\xi_k\cos n\omega_k t+i\xi_k\sin n\omega_k$$

$E X ( n ) = E\sum _ { k = 0 } ^ { + \infty }\xi_k  e ^ { i n w_k } = 0$

$R _ { X } ( n , n + m ) = E ( \sum _ { k = 0 } ^ { + \infty } \xi _ { k } e ^ { i n \omega_k } )\overline{ ( \sum _ { l = 0 } ^ { + \infty } \xi _ { l } e ^ { i ( n + m ) \omega_l } )}$

$= E ( \sum _ { k = 0 } ^ { + \infty } \xi _ { k } e ^ { i n \omega_k } ) ( \sum _ { l = 0 } ^ { + \infty } \xi _ { l } e ^ {- i ( n + m ) \omega_l } )$

$= \sum _ { k = 0 } ^ { + \infty } \sigma _ { k } ^ { 2 } e ^ {-i m \omega_k } = R _ { x } ( m ) .$



35.

$\left|R_{X}(t)\right|=\left|E X_{(t+\tau)} X_{(t)}\right| \leqslant\left|E X_{(t+\tau)}^{2}\right|^{1 / 2}\left|E X_{(t)}^{2}\right|^{1 / 2}$ 
$=\left|R_{X}(0)\right|^{1 / 2}\left|R_{X(0)}\right|^{1 / 2}=R_{X}(0)$
$R_{X}(\tau)=E X_{(t)} X_{(t+\tau)}=E X_{(t+\tau)} X_{(t)}=R_{X}(-\tau)$



36.

时间平均.$<X(t)>=\lim_{T\rightarrow\infty}\frac{1}{2T}\int_{-T}^{T}X(t)dt$. $m_X$
时间相关函数.$<X(t)X(t+\tau)>=\lim_{T\rightarrow\infty}\frac{1}{2T}\int_{-T}^{T}X(t)X(t+\tau)dt$
$P(<X(t)>=m_X)=1$, $<X(t)>=m_X$ a.s. $R_X(\tau)$
$m_X(t)=0$
$R_X(t,t+\tau)=\frac{a^2}{2}\cos\omega_0\tau=R_X(\tau)$

$<X(t)>=lim_{T\rightarrow\infty}\frac{1}{2T}\int_{-T}^{T}X(t)dt=lim_{T\rightarrow\infty}\frac{1}{2T}\int_{-T}^{T}a\cos(\omega_0t+\Phi)dt$
$
=lim_{T\rightarrow\infty}\frac{a}{2T}\int_{-T}^{T}(\cos(\omega_0t+\cos\Phi)-\sin\omega_0t\sin\Phi)dt$
$=lim_{T\rightarrow\infty}\frac{a}{2T}(\cos\Phi\int_{-T}^{T}\cos\omega_0tdt-\sin\Phi\int_{-T}^{T}\sin\omega_0tdt)$

$= \lim_{T \to \infty} \frac{a}{2T}  \frac{2}{\omega_0} \sin (\omega_0T) \cos \Phi$
$= \lim_{T \to \infty} \frac{a \sin (\omega_0T)}{T\omega_0} \cdot \cos \Phi$

$=0$

$<X(t),X(t+\tau)>=\lim_{T\rightarrow\infty}\frac{1}{2T}\int_{-T}^{T}X(t)X(t+\tau)d\tau$
$
=\lim_{T\rightarrow\infty}\frac{1}{2T}\int_{-T}^{T}a^{2}\cos(\omega_{0}t+\Phi)\cos(\omega_{0}(t+\tau)+\Phi)dt$

$=\frac{a^2}{2}\cos\omega_0\tau$



37.

$\lim_{T \to \infty} \frac{1}{T} \int_0^{2T} (1 - \frac{\tau}{2T})(R_X(\tau) - m_X^2) d\tau$  
$= \lim_{T \to \infty} \frac{1}{T} \int_0^{2T} (1 - \frac{\tau}{2T}) \dot{\sigma}^2 \cos\omega_0 \tau d\tau$  
$= \lim_{T \to \infty} \frac{\dot{\sigma}^2}{T}\frac{1}{\omega_0} \int_0^{2T} (1 - \frac{\tau}{2T}) d\sin\omega_0 \tau$  
$= \lim_{T \to \infty} \frac{\dot{\sigma}^2}{T\omega_0} \left( (1 - \frac{\tau}{2T}) \sin\omega_0 \tau \Big|_0^{2T} + \int_0^{2T} \sin\omega_0 \tau \frac{1}{2T} d\tau \right)$

$=\lim_{T\to\infty}\frac{\sigma^{2}}{T\omega_0}\cdot\frac{1}{2T}\cdot\frac{1}{\omega_0}(-\cos\omega_{0}\tau)\Big|_0^{2T}$

38.

$R_X(\tau) = \frac{1}{2\pi} \int_{-\infty}^{+\infty} e^{i\omega \tau} S_X(\omega) d\omega=\frac{1}{\pi}\int_{0}^{+\infty}\cos w \tau S_X(\omega)dw$

$S_X(\omega) = \int_{-\infty}^{+\infty} e^{-i\omega \tau} R_X(\tau) d\omega = \int_{-\infty}^{+\infty} \cos\omega \tau R_X(\tau) d\tau - i\int_{-\infty}^{+\infty} \sin\omega \tau R_X(\tau) d\tau$

$=\int_{-\infty}^{+\infty} \cos\omega \tau R_X(\tau) d\tau$

$=2\int_{0}^{+\infty} \cos\omega \tau R_X(\tau) d\tau$

$S_X(\omega) = \lim_{T \to \infty} \frac{1}{2T} E|F(w,T)|^2\geq0$



39.

$R_X(\tau)=\frac{1}{2\pi}\int_{-\infty}^{+\infty}\delta(\omega)e^{i\omega \tau}dw=\frac{1}{2\pi}e^{i0\tau}=\frac{1}{2\pi}$

$S_X(w)=\int_{-\infty}^{+\infty}e^{-i\omega \tau}\cdot S_0\delta(\tau)d\tau=S_0$



40.

$S _ { X } ( w ) = \sigma^2 \int _ { - \infty } ^ { + \infty } \cos w _ { 0 } \tau \cdot e ^ { - i w \tau } d \tau$
$= \sigma ^ { 2 } \int _ { - \infty } ^ { + \infty } \frac { e ^ { i w_0 \tau } + e ^ { - i w_0 \tau } } { 2 } e ^ { - i w \tau } d \tau$
$= \frac { \sigma ^ { 2 } } { 2 } \int _ { - \infty } ^ { + \infty } e ^ { - i ( w - w _ { 0 } ) \tau } d \tau + \int _ { - \infty } ^ { + \infty } e ^ { - i ( w + w _ { 0 } ) \tau } d \tau$

$由于\mathscr{F} _ { 1 } [ 1 ] = 2 \pi \delta ( \omega ) = \int _ { - \infty } ^ { + \infty } 1 \cdot e ^ { - i \omega \tau } d \tau$

$=\frac { \sigma ^ { 2 } } { 2 }[2\pi\delta(\omega-\omega_{0})]-2\pi\delta(\omega+\omega_{0})]$

$\mathscr{F}_{1}[\cos \omega_{0}\tau]=\pi[\delta(\omega-\omega_{0})+\delta(\omega+\omega_{0})]$



41.

$S _ { X } ( w ) = I^2 \int _ { - \infty } ^ { + \infty } e ^ { - 2 \lambda \vert \tau \vert } \cdot e ^ { - i w \tau } d \tau$

$= I ^ { 2 } ( \int _ { - \infty } ^ { 0 } e ^ { ( 2 \lambda - i w ) \tau } d \tau + \int _ { 0 } ^ { + \infty } e ^ { -( 2 \lambda + i w ) \tau } d \tau )$

$= I ^ { 2 } ( \frac { 1 } { 2 \lambda - i w } e ^ { ( 2 \lambda - i w ) \tau } \vert _ { - \infty } ^ { 0 } + ( -\frac { 1 } { 2 \lambda + i w } ) e ^ { -( 2 \lambda + i w ) \tau } \vert _ { 0 } ^ { + \infty } )$

$= I ^ { 2 } ( \frac { 1 } { 2 \lambda - i w } + \frac { 1 } { 2 \lambda + i w } ) = I ^ { 2 } \frac { 4 \lambda } { 4 \lambda ^ { 2 } + w ^ { 2 } }$

$\mathscr{F}[e^{-a|\tau|}]=\frac{2\times a}{a^{2}+\omega^{2}}$



42.

$\frac{w^2+4}{w^4+10w^2+9} = \frac{w^2+1}{(w^2+9)(w^2+1)}$
$
= \frac{\frac{5}{8}}{w^2+9} + \frac{\frac{3}{8}}{w^2+1}$
$\mathcal{F}^{-1} \left[\frac{\frac{5}{8}}{w^2+9}\right] = \mathcal{F}^{-1} \left[\frac{2 \times 3}{w^2+3^2} \times \frac{5}{48}\right] = \frac{5}{48} e^{-3 |\tau|}$

$\mathcal{F}^{-1} \left[\frac{\frac{3}{8}}{w^2+1}\right] = \mathcal{F}^{-1} \left[\frac{2 \times 1}{w^2+1} \times \frac{3}{16}\right] = \frac{3}{16} e^{- |\tau|}$



43.

$\mathscr{F}\left[ {f\left( \tau \right)\cos \omega _0 \tau } \right]$ 
$= \int_{ - \infty }^{ + \infty } {f\left( \tau \right)\cos \omega _0 \tau \cdot e^{ - i\omega \tau } d\tau }$
$= \int_{ - \infty }^{ + \infty } {f\left( \tau \right)\frac{{{e^{i\omega _0 \tau }} + {e^{ - i\omega _0 \tau }}}}{{2}} \cdot e^{ - i\omega \tau } d\tau }$
$= \frac{1}{2}( \int_{ - \infty }^{ + \infty } {f\left( \tau \right) \cdot {e^{ - i\left( {\omega - \omega _0 } \right)\tau }}d\tau } + \int_{ - \infty }^{ + \infty } {f\left( \tau \right) \cdot {e^{-i\left( {\omega + \omega _0 } \right)\tau }}d\tau })$
$= \frac{1}{2}\left( {F\left( {\omega - \omega _0 } \right) + F\left( {\omega + \omega _0 } \right)} \right)$

$\int_{-\infty}^{+\infty}f(\tau)e^{-i\omega\tau}d\tau=\mathscr{F}[f(\tau)] = F(\omega)$

$\mathscr{F}[e^{-a|\tau|}]=\frac{2a}{a^2 + \omega^2}$



44.

$\mathscr F ^ { - 1 } [ S _ { x } ( w ) = \frac { 1 } { ( 1 + w ^ { 2 } ) ^ { 2 } } ]\Rightarrow \mathscr F ^ { - 1 } [ \frac { 1 } { 1 + w ^ { 2 } } \cdot \frac { 1 } { 1 + w ^ { 2 } } ] = R _ { Y } ( \tau ) * R _ { Y } ( \tau )$
$
\mathscr F ^ { - 1 } [ \frac { 1 } { 2 } \frac { 2 \times 1 } { 1 + w ^ { 2 } } ] = \frac { 1 } { 2 } e ^ { - \mid \tau \mid } = R _ { Y } ( \tau )$
$设\tau \geq 0$
$R _ { X }=R _ { Y } ( \tau ) * R _ { Y } ( \tau )= \int _ { - \infty } ^ { + \infty } R _ { Y } ( u ) R _ { Y } ( \tau - u ) d u = \frac { 1 } { 4 } \int _ { - \infty } ^ { + \infty } e ^ { - \mid u \mid } e ^ { - \mid \tau - u \mid } d u$

$=\frac{1}{4}(\int_{-\infty}^{0}e^ue^{-(\tau-u)}du+\int_{0}^{\tau}e^{-u}e^{-(\tau-u)}du+\int_{\tau}^{+\infty}e^{-u}e^{-(\tau-u)}du)$

$
=\frac{1}{4}(\frac{1}{2}e^{-\tau}+\tau e^{-\tau}+\frac{1}{2}e^{-\tau})=\frac{1}{4}(e^{-\tau}+\tau e^{-\tau})$

$R_{X}(-\tau)=R_{X}(\tau)=\frac{1}{4}(e^{-\tau}+\tau e^{-\tau})$
$
R_{X}(\tau)=\frac{1}{4}(e^{-|\tau|}+|\tau|e^{-|\tau|})$